NoveltyTheory/All.lean
@@ -15,6 +15,7 @@ import NoveltyTheory.Models.BoundedRegimeDiagonal
 import NoveltyTheory.Models.ReducerDiagonal
 import NoveltyTheory.Models.CausalExplanatoryOrders
 import NoveltyTheory.Models.GenCertPhase
+import NoveltyTheory.Models.SimulationVersusExplanation
 import NoveltyTheory.Ridge.ShiftWitness
 import NoveltyTheory.Ridge.DiagonalNat
 import NoveltyTheory.Ridge.InterfaceAlignment
